fix Pcmpl,Pimull_r

autogen/EncDecRet.v
@@ -1,6 +1,6 @@
 Require Import Coqlib Integers Errors.
 Require Import encode.Hex encode.Bits Memdata.
-Require Import Encode  VerificationCondition.
+Require Import Encode VerificationCondition.
 Import String Ascii.
 Import List.
 Import ListNotations.
@@ -278,7 +278,7 @@ Hint Unfold read_B write_B read_R write_R read_W write_W read_X write_X read_bas
 
 Hint Unfold AddrE12_bp AddrE11_bp AddrE10_bp AddrE9_bp AddrE8_bp AddrE7_bp AddrE6_bp AddrE5_bp AddrE4_bp AddrE0_bp :AddrE_bpdb.
 
-Hint Unfold Ptestq_EvGv_bp Ptestq_ri_bp Pcmpq_GvEv_bp Pcmpq_EvGv_bp Pcmpq_ri_bp Prorq_ri_bp Psarq_ri_bp Psarq_rcl_bp Psalq_ri_bp Psalq_rcl_bp Pnotq_bp Pxorq_GvEv_bp Pxorq_EvGv_bp Pxorq_ri_bp Porq_GvEv_bp Porq_EvGv_bp Porq_ri_bp Pandq_GvEv_bp Pandq_EvGv_bp Pandq_ri_bp Pdivq_bp Pidivq_bp Pmulq_r_bp Pimulq_GvEv_bp Pimulq_r_bp Pimulq_ri_bp Psubq_GvEv_bp Psubq_EvGv_bp Psubq_ri_bp Paddq_GvEv_bp Paddq_EvGv_bp Paddq_ri_bp Pnegq_bp Pleaq_bp Pmovq_EvGv_bp Pmovq_GvEv_bp Pmovq_ri_bp Psubl_ri_bp Pbsqrtsd_bp Psbbl_rr_bp Prep_movsl_bp Pmovsq_rm_bp Pmovsq_mr_bp Pminsd_bp Pmaxsd_bp Pbswap32_bp Pbsrl_bp Pbsfl_bp Paddl_mi_bp Paddl_rr_bp Padcl_rr_bp Padcl_ri_bp Pjcc_rel_bp Pret_iw_bp Pret_bp Pcall_r_bp Pcall_ofs_bp Pnop_bp Pjmp_Ev_bp Pjmp_l_rel_bp Pandps_fm_bp Pxorps_GvEv_bp Pxorpd_GvEv_bp Pcomiss_ff_bp Pcomisd_ff_bp Pdivss_ff_bp Pdivsd_ff_bp Pmuls_ff_bp Pmuld_ff_bp Psubs_ff_bp Psubd_ff_bp Padds_ff_bp Paddd_ff_bp Psetcc_bp Pcmov_bp Ptestl_rr_bp Ptestl_ri_bp Pcmpl_ri_bp Pcmpl_rr_bp Prorl_ri_bp Prolw_ri_bp Pshld_ri_bp Psarl_rcl_bp Psarl_ri_bp Pshrl_rcl_bp Pshrl_ri_bp Psall_rcl_bp Psall_ri_bp Pnotl_bp Pxorl_rr_bp Pxorl_ri_bp Porl_rr_bp Porl_ri_bp Pandl_ri_bp Pandl_rr_bp Pidivl_r_bp Pdivl_r_bp Pcltd_bp Pmull_r_bp Pimull_ri_bp Pimull_rr_bp Psubl_rr_bp Paddl_ri_bp Pnegl_bp Pleal_bp Pcvttss2si_rf_bp Pcvtsi2sd_fr_bp Pcvtsi2ss_fr_bp Pcvttsd2si_rf_bp Pcvtss2sd_ff_bp Pcvtsd2ss_ff_bp Pmovsw_GvEv_bp Pmovzw_GvEv_bp Pmovsb_GvEv_bp Pmovzb_rm_bp Pmovw_rm_bp Pmovw_mr_bp Pmovb_rm_bp Pmovb_mr_bp Pxchg_rr_bp Pflds_m_bp Pfstps_m_bp Pfstpl_m_bp Pfldl_m_bp Pmovss_fm_bp Pmovss_mf_bp Pmovsd_fm_bp Pmovsd_mf_bp Pmovl_rm_bp Pmovl_mr_bp Pmovl_ri_bp :Instruction_bpdb.
+Hint Unfold Ptestq_EvGv_bp Ptestq_ri_bp Pcmpq_GvEv_bp Pcmpq_EvGv_bp Pcmpq_ri_bp Prorq_ri_bp Psarq_ri_bp Psarq_rcl_bp Psalq_ri_bp Psalq_rcl_bp Pnotq_bp Pxorq_GvEv_bp Pxorq_EvGv_bp Pxorq_ri_bp Porq_GvEv_bp Porq_EvGv_bp Porq_ri_bp Pandq_GvEv_bp Pandq_EvGv_bp Pandq_ri_bp Pdivq_bp Pidivq_bp Pmulq_r_bp Pimulq_GvEv_bp Pimulq_r_bp Pimulq_ri_bp Psubq_GvEv_bp Psubq_EvGv_bp Psubq_ri_bp Paddq_GvEv_bp Paddq_EvGv_bp Paddq_ri_bp Pnegq_bp Pleaq_bp Pmovq_EvGv_bp Pmovq_GvEv_bp Pmovq_ri_bp Psubl_ri_bp Pbsqrtsd_bp Psbbl_rr_bp Prep_movsl_bp Pmovsq_rm_bp Pmovsq_mr_bp Pminsd_bp Pmaxsd_bp Pbswap32_bp Pbsrl_bp Pbsfl_bp Paddl_mi_bp Paddl_rr_bp Padcl_rr_bp Padcl_ri_bp Pjcc_rel_bp Pret_iw_bp Pret_bp Pcall_r_bp Pcall_ofs_bp Pnop_bp Pjmp_Ev_bp Pjmp_l_rel_bp Pandps_fm_bp Pxorps_GvEv_bp Pxorpd_GvEv_bp Pcomiss_ff_bp Pcomisd_ff_bp Pdivss_ff_bp Pdivsd_ff_bp Pmuls_ff_bp Pmuld_ff_bp Psubs_ff_bp Psubd_ff_bp Padds_ff_bp Paddd_ff_bp Psetcc_bp Pcmov_bp Ptestl_rr_bp Ptestl_ri_bp Pcmpl_ri_bp Pcmpl_rr_bp Prorl_ri_bp Prolw_ri_bp Pshld_ri_bp Psarl_rcl_bp Psarl_ri_bp Pshrl_rcl_bp Pshrl_ri_bp Psall_rcl_bp Psall_ri_bp Pnotl_bp Pxorl_rr_bp Pxorl_ri_bp Porl_rr_bp Porl_ri_bp Pandl_ri_bp Pandl_rr_bp Pidivl_r_bp Pdivl_r_bp Pcltd_bp Pmull_r_bp Pimull_r_bp Pimull_ri_bp Pimull_rr_bp Psubl_rr_bp Paddl_ri_bp Pnegl_bp Pleal_bp Pcvttss2si_rf_bp Pcvtsi2sd_fr_bp Pcvtsi2ss_fr_bp Pcvttsd2si_rf_bp Pcvtss2sd_ff_bp Pcvtsd2ss_ff_bp Pmovsw_GvEv_bp Pmovzw_GvEv_bp Pmovsb_GvEv_bp Pmovzb_rm_bp Pmovw_rm_bp Pmovw_mr_bp Pmovb_rm_bp Pmovb_mr_bp Pxchg_rr_bp Pflds_m_bp Pfstps_m_bp Pfstpl_m_bp Pfldl_m_bp Pmovss_fm_bp Pmovss_mf_bp Pmovsd_fm_bp Pmovsd_mf_bp Pmovl_rm_bp Pmovl_mr_bp Pmovl_ri_bp :Instruction_bpdb.
 Lemma AddrE_bp_in_list0: 
 In AddrE12_bp AddrE_bp_list.
 Proof.
@@ -825,161 +825,166 @@ Proof.
 simpl; goOver; auto. Qed.
 
 Lemma Instruction_bp_in_list99: 
-In Pimull_ri_bp Instruction_bp_list.
+In Pimull_r_bp Instruction_bp_list.
 Proof.
 simpl; goOver; auto. Qed.
 
 Lemma Instruction_bp_in_list100: 
-In Pimull_rr_bp Instruction_bp_list.
+In Pimull_ri_bp Instruction_bp_list.
 Proof.
 simpl; goOver; auto. Qed.
 
 Lemma Instruction_bp_in_list101: 
-In Psubl_rr_bp Instruction_bp_list.
+In Pimull_rr_bp Instruction_bp_list.
 Proof.
 simpl; goOver; auto. Qed.
 
 Lemma Instruction_bp_in_list102: 
-In Paddl_ri_bp Instruction_bp_list.
+In Psubl_rr_bp Instruction_bp_list.
 Proof.
 simpl; goOver; auto. Qed.
 
 Lemma Instruction_bp_in_list103: 
-In Pnegl_bp Instruction_bp_list.
+In Paddl_ri_bp Instruction_bp_list.
 Proof.
 simpl; goOver; auto. Qed.
 
 Lemma Instruction_bp_in_list104: 
-In Pleal_bp Instruction_bp_list.
+In Pnegl_bp Instruction_bp_list.
 Proof.
 simpl; goOver; auto. Qed.
 
 Lemma Instruction_bp_in_list105: 
-In Pcvttss2si_rf_bp Instruction_bp_list.
+In Pleal_bp Instruction_bp_list.
 Proof.
 simpl; goOver; auto. Qed.
 
 Lemma Instruction_bp_in_list106: 
-In Pcvtsi2sd_fr_bp Instruction_bp_list.
+In Pcvttss2si_rf_bp Instruction_bp_list.
 Proof.
 simpl; goOver; auto. Qed.
 
 Lemma Instruction_bp_in_list107: 
-In Pcvtsi2ss_fr_bp Instruction_bp_list.
+In Pcvtsi2sd_fr_bp Instruction_bp_list.
 Proof.
 simpl; goOver; auto. Qed.
 
 Lemma Instruction_bp_in_list108: 
-In Pcvttsd2si_rf_bp Instruction_bp_list.
+In Pcvtsi2ss_fr_bp Instruction_bp_list.
 Proof.
 simpl; goOver; auto. Qed.
 
 Lemma Instruction_bp_in_list109: 
-In Pcvtss2sd_ff_bp Instruction_bp_list.
+In Pcvttsd2si_rf_bp Instruction_bp_list.
 Proof.
 simpl; goOver; auto. Qed.
 
 Lemma Instruction_bp_in_list110: 
-In Pcvtsd2ss_ff_bp Instruction_bp_list.
+In Pcvtss2sd_ff_bp Instruction_bp_list.
 Proof.
 simpl; goOver; auto. Qed.
 
 Lemma Instruction_bp_in_list111: 
-In Pmovsw_GvEv_bp Instruction_bp_list.
+In Pcvtsd2ss_ff_bp Instruction_bp_list.
 Proof.
 simpl; goOver; auto. Qed.
 
 Lemma Instruction_bp_in_list112: 
-In Pmovzw_GvEv_bp Instruction_bp_list.
+In Pmovsw_GvEv_bp Instruction_bp_list.
 Proof.
 simpl; goOver; auto. Qed.
 
 Lemma Instruction_bp_in_list113: 
-In Pmovsb_GvEv_bp Instruction_bp_list.
+In Pmovzw_GvEv_bp Instruction_bp_list.
 Proof.
 simpl; goOver; auto. Qed.
 
 Lemma Instruction_bp_in_list114: 
-In Pmovzb_rm_bp Instruction_bp_list.
+In Pmovsb_GvEv_bp Instruction_bp_list.
 Proof.
 simpl; goOver; auto. Qed.
 
 Lemma Instruction_bp_in_list115: 
-In Pmovw_rm_bp Instruction_bp_list.
+In Pmovzb_rm_bp Instruction_bp_list.
 Proof.
 simpl; goOver; auto. Qed.
 
 Lemma Instruction_bp_in_list116: 
-In Pmovw_mr_bp Instruction_bp_list.
+In Pmovw_rm_bp Instruction_bp_list.
 Proof.
 simpl; goOver; auto. Qed.
 
 Lemma Instruction_bp_in_list117: 
-In Pmovb_rm_bp Instruction_bp_list.
+In Pmovw_mr_bp Instruction_bp_list.
 Proof.
 simpl; goOver; auto. Qed.
 
 Lemma Instruction_bp_in_list118: 
-In Pmovb_mr_bp Instruction_bp_list.
+In Pmovb_rm_bp Instruction_bp_list.
 Proof.
 simpl; goOver; auto. Qed.
 
 Lemma Instruction_bp_in_list119: 
-In Pxchg_rr_bp Instruction_bp_list.
+In Pmovb_mr_bp Instruction_bp_list.
 Proof.
 simpl; goOver; auto. Qed.
 
 Lemma Instruction_bp_in_list120: 
-In Pflds_m_bp Instruction_bp_list.
+In Pxchg_rr_bp Instruction_bp_list.
 Proof.
 simpl; goOver; auto. Qed.
 
 Lemma Instruction_bp_in_list121: 
-In Pfstps_m_bp Instruction_bp_list.
+In Pflds_m_bp Instruction_bp_list.
 Proof.
 simpl; goOver; auto. Qed.
 
 Lemma Instruction_bp_in_list122: 
-In Pfstpl_m_bp Instruction_bp_list.
+In Pfstps_m_bp Instruction_bp_list.
 Proof.
 simpl; goOver; auto. Qed.
 
 Lemma Instruction_bp_in_list123: 
-In Pfldl_m_bp Instruction_bp_list.
+In Pfstpl_m_bp Instruction_bp_list.
 Proof.
 simpl; goOver; auto. Qed.
 
 Lemma Instruction_bp_in_list124: 
-In Pmovss_fm_bp Instruction_bp_list.
+In Pfldl_m_bp Instruction_bp_list.
 Proof.
 simpl; goOver; auto. Qed.
 
 Lemma Instruction_bp_in_list125: 
-In Pmovss_mf_bp Instruction_bp_list.
+In Pmovss_fm_bp Instruction_bp_list.
 Proof.
 simpl; goOver; auto. Qed.
 
 Lemma Instruction_bp_in_list126: 
-In Pmovsd_fm_bp Instruction_bp_list.
+In Pmovss_mf_bp Instruction_bp_list.
 Proof.
 simpl; goOver; auto. Qed.
 
 Lemma Instruction_bp_in_list127: 
-In Pmovsd_mf_bp Instruction_bp_list.
+In Pmovsd_fm_bp Instruction_bp_list.
 Proof.
 simpl; goOver; auto. Qed.
 
 Lemma Instruction_bp_in_list128: 
-In Pmovl_rm_bp Instruction_bp_list.
+In Pmovsd_mf_bp Instruction_bp_list.
 Proof.
 simpl; goOver; auto. Qed.
 
 Lemma Instruction_bp_in_list129: 
-In Pmovl_mr_bp Instruction_bp_list.
+In Pmovl_rm_bp Instruction_bp_list.
 Proof.
 simpl; goOver; auto. Qed.
 
 Lemma Instruction_bp_in_list130: 
+In Pmovl_mr_bp Instruction_bp_list.
+Proof.
+simpl; goOver; auto. Qed.
+
+Lemma Instruction_bp_in_list131: 
 In Pmovl_ri_bp Instruction_bp_list.
 Proof.
 simpl; goOver; auto. Qed.
@@ -1407,6 +1412,7 @@ Inductive Instruction: Type :=
 | Pdivl_r(uvar3_0:u3)
 | Pcltd
 | Pmull_r(uvar3_0:u3)
+| Pimull_r(uvar3_0:u3)
 | Pimull_ri(uvar3_0:u3)(uvar3_1:u3)(uvar32_2:u32)
 | Pimull_rr(uvar3_0:u3)(uvar3_1:u3)
 | Psubl_rr(uvar3_0:u3)(uvar3_1:u3)
@@ -1539,6 +1545,7 @@ Inductive Instruction_op: Type :=
 | Pdivl_r_op
 | Pcltd_op
 | Pmull_r_op
+| Pimull_r_op
 | Pimull_ri_op
 | Pimull_rr_op
 | Psubl_rr_op
@@ -1672,6 +1679,7 @@ Definition Instruction_to_op element  :=
 | Pdivl_r _ => Pdivl_r_op
 | Pcltd => Pcltd_op
 | Pmull_r _ => Pmull_r_op
+| Pimull_r _ => Pimull_r_op
 | Pimull_ri _ _ _ => Pimull_ri_op
 | Pimull_rr _ _ => Pimull_rr_op
 | Psubl_rr _ _ => Psubl_rr_op
@@ -1806,6 +1814,7 @@ Definition Instruction_op_to_bp element  :=
 | Pdivl_r_op => Pdivl_r_bp
 | Pcltd_op => Pcltd_bp
 | Pmull_r_op => Pmull_r_bp
+| Pimull_r_op => Pimull_r_bp
 | Pimull_ri_op => Pimull_ri_bp
 | Pimull_rr_op => Pimull_rr_bp
 | Psubl_rr_op => Psubl_rr_bp
@@ -2959,6 +2968,14 @@ let result0 := [byte01] in
 let byte10 := HB["00"] in
 let byte11 := write_mod byte10 b["11"] in
 let byte12 := write_reg_op byte11 b["100"] in
+let byte13 := write_rm byte12 (proj1_sig uvar3_0) in
+let result1 := [byte13] in
+OK (result0 ++ result1)
+| Pimull_r uvar3_0 => let byte01 := HB["F7"] in
+let result0 := [byte01] in
+let byte10 := HB["00"] in
+let byte11 := write_mod byte10 b["11"] in
+let byte12 := write_reg_op byte11 b["101"] in
 let byte13 := write_rm byte12 (proj1_sig uvar3_0) in
 let result1 := [byte13] in
 OK (result0 ++ result1)
@@ -4936,6 +4953,17 @@ let uvar3_0 := read_rm byte0 in
 if assertLength uvar3_0 3 then
 do bytes2 <- try_skip_n bytes1 1;
 OK ((Pmull_r (uvar3_0)), 2)
+else Error(msg"impossible")
+else
+
+	if Pimull_r_bp bin then
+let bytes0 := code in
+do bytes1 <- try_skip_n bytes0 1;
+do byte0 <- try_get_n bytes1 0;
+let uvar3_0 := read_rm byte0 in
+if assertLength uvar3_0 3 then
+do bytes2 <- try_skip_n bytes1 1;
+OK ((Pimull_r (uvar3_0)), 2)
 else Error(msg"impossible")
 else
 
